src/sort/ternaryComparisonsScript.sml
@@ -1,19 +1,8 @@
-open HolKernel Parse boolLib listTheory
-     TotalDefn Datatype BasicProvers;
+open HolKernel Parse boolLib bossLib;
 
-infix THEN THENL |->;
+val _ = new_theory "ternaryComparisons";
 
-val _ = new_theory "prelim";
-
-
-(* ternary comparisons *)
-
-val _ = Hol_datatype `ordering = LESS | EQUAL | GREATER`;
-
-val compare_def = Define `
-   (compare LESS    lt eq gt = lt)
-/\ (compare EQUAL   lt eq gt = eq)
-/\ (compare GREATER lt eq gt = gt) `
+val _ = Datatype `ordering = LESS | EQUAL | GREATER`;
 
 fun type_rws ty = #rewrs (TypeBase.simpls_of ty)
 
@@ -26,17 +15,32 @@ val ordering_eq_dec = save_thm("ordering_eq_dec",
   PURE_REWRITE_RULE[GSYM (hd (rev (CONJUNCTS (SPEC_ALL EQ_CLAUSES))))] thms);
 
 
-(* General results on lists *)
+(* Lifting comparison functions through various type operators *)
+val pair_compare_def = Define`
+  pair_compare c1 c2 (a,b) (x,y) =
+     case c1 a x of
+        EQUAL => c2 b y
+      | res => res
+`;
 
+val option_compare_def = Define`
+  (option_compare c NONE NONE = EQUAL) /\
+  (option_compare c NONE (SOME _) = LESS) /\
+  (option_compare c (SOME _) NONE = GREATER) /\
+  (option_compare c (SOME v1) (SOME v2) = c v1 v2)
+`;
+
+
+(* General results on lists *)
 val list_compare_def = Define `
    (list_compare cmp [] [] = EQUAL)
 /\ (list_compare cmp [] l2 = LESS)
 /\ (list_compare cmp l1 [] = GREATER)
 /\ (list_compare cmp (x::l1) (y::l2) =
-     compare (cmp (x:'a) y)
-     (* x<y *) LESS
-     (* x=y *) (list_compare cmp l1 l2)
-     (* x>y *) GREATER) `;
+     case cmp (x:'a) y of
+       LESS => LESS
+     | EQUAL => list_compare cmp l1 l2
+     | GREATER => GREATER) `;
 
 val compare_equal = store_thm("compare_equal",
   --` (!x y. (cmp x y = EQUAL) = (x = y))
@@ -44,8 +48,9 @@ val compare_equal = store_thm("compare_equal",
  DISCH_THEN (ASSUME_TAC o GSYM)
    THEN NTAC 2 (Induct THENL [ALL_TAC,GEN_TAC])
    THEN TRY (ASM_REWRITE_TAC[] THEN Cases_on `cmp h h'`)
-   THEN RW_TAC bool_ss [list_compare_def, compare_def]);
+   THEN RW_TAC bool_ss [list_compare_def]);
 
+(* looks out of place *)
 val list_merge_def = Define `
    (list_merge a_lt l1 [] = l1)
 /\ (list_merge a_lt [] l2 = l2)
@@ -53,6 +58,5 @@ val list_merge_def = Define `
       if a_lt x y
       then x::list_merge a_lt l1 (y::l2)
       else y::list_merge a_lt (x::l1) l2) `;
-
 
 val _ = export_theory();
